tried a different approach to building instances for imports... which also did not succeed

examples/Test.v
@@ -57,71 +57,31 @@ Check (toIsoInterp
 Spec End GroupTest.
 
 
-Definition mon_T__repr_instance (ops:spec_ops Monoid.Monoid__repr) : Monoid.T__class :=
-  ops_head ops.
-Definition mon_m_zero__repr_instance (ops:spec_ops Monoid.Monoid__repr)
-: Monoid.m_zero__class :=
-  ops_head (ops_rest ops).
-Definition mon_m_plus__repr_instance (ops:spec_ops Monoid.Monoid__repr)
-: Monoid.m_plus__class :=
-  ops_head (ops_rest (ops_rest ops)).
 
-Definition mon_mk_ops T__param m_zero__param m_plus__param :
-  spec_ops Monoid.Monoid__repr :=
-  ops_cons
-    T__param (I : sats_op_pred None _)
-    (ops_cons
-       m_zero__param (I : sats_op_pred None _)
-       (ops_cons
-          m_plus__param (I : sats_op_pred None _)
-          (tt : spec_ops (Spec_Axioms _)))).
+Class mon_ops : Type :=
+  mon_spec_ops : spec_ops Monoid.Monoid__repr.
+Class mon_model {ops:mon_ops} : Prop :=
+  mon_spec_model : spec_model Monoid.Monoid__repr mon_spec_ops.
 
-Definition mon_spec_repr__instance__H
-           T__param m_zero__param m_plus__param
-           (* (mod: spec_model _ (mon_mk_ops T__param m_zero__param m_plus__param)) *)
-           (mod: Monoid.m_zero_left__class /\
-                 (Monoid.m_zero_right__class /\ Monoid.m_plus_assoc__class)) :
-  @Monoid.Monoid T__param m_zero__param m_plus__param :=
-  {| Monoid.m_zero_left__axiom := proj1 mod;
-        Monoid.m_zero_right__axiom := proj1 (proj2 mod);
-        Monoid.m_plus_assoc__axiom := proj2 (proj2 mod) |}.
+Instance mon_T__instance `{mon_ops} : Monoid.T__class :=
+  ops_head mon_spec_ops.
+Instance mon_m_zero__instance `{mon_ops} : Monoid.m_zero__class :=
+  ops_head (ops_rest mon_spec_ops).
+Instance mon_m_plus__instance `{mon_ops} : Monoid.m_plus__class :=
+  ops_head (ops_rest (ops_rest mon_spec_ops)).
 
-Definition mon_spec_repr__instance
-           T__param m_zero__param m_plus__param
-           (mod: spec_model _ (mon_mk_ops T__param m_zero__param m_plus__param)) :
-  @Monoid.Monoid T__param m_zero__param m_plus__param :=
-  mon_spec_repr__instance__H _ _ _ mod.
-
-
-(*
-Definition mon_spec_repr__instance2
-           T__param m_zero__param m_plus__param
-           (mod: spec_model
-                   _
-                   (ops_cons
-                      T__param (I : sats_op_pred None _)
-                      (ops_cons
-                         m_zero__param (I : sats_op_pred None _)
-                         (ops_cons
-                            m_plus__param (I : sats_op_pred None _)
-                            (tt : spec_ops (Spec_Axioms _)))))) :
-  @Monoid.Monoid T__param m_zero__param m_plus__param :=
-  mon_spec_repr__instance__H _ _ _ mod.
-*)
-
-Definition mon_spec_repr__instance2
-           T__param m_zero__param m_plus__param
-           (mod: spec_model _ (mon_mk_ops T__param m_zero__param m_plus__param)) :
-  @Monoid.Monoid T__param m_zero__param m_plus__param :=
-  mon_spec_repr__instance__H _ _ _ mod.
-
-(*
-Definition mon_e_model T__param m_zero__param m_plus__param :
-  spec_model _ (mon_mk_ops T__param m_zero__param m_plus__param) =
-  Monoid.m_zero_left__class /\
-  (Monoid.m_zero_right__class /\ Monoid.m_plus_assoc__class) :=
-  eq_refl.
-*)
+Instance mon__instance `{mon_model} : Monoid.Monoid.
+revert ops H.
+unfold mon_ops; unfold mon_model; unfold Monoid.Monoid__repr.
+intro ops.
+repeat (let t := fresh "t" in
+        let pf := fresh "pf" in
+        destruct ops as [t ops]; destruct ops as [pf ops];
+        try destruct pf).
+compute.
+intro H; repeat (let Hi := fresh "H" in
+                 destruct H as [Hi H]); constructor; assumption.
+Qed.
 
 
 Definition grp_repr__ops `{GroupTest.GroupTest} : spec_ops GroupTest.GroupTest__repr :=
@@ -135,7 +95,12 @@ Definition grp_repr__ops `{GroupTest.GroupTest} : spec_ops GroupTest.GroupTest__
              m_inv__param (I : sats_op_pred None _)
              (tt : spec_ops (Spec_Axioms _))))).
 
-
+Definition grp_repr__model `{GroupTest.GroupTest} :
+  spec_model GroupTest.GroupTest__repr grp_repr__ops.
+  compute.
+  destruct H.
+  repeat (first [ assumption | split; [assumption|] | apply I]).
+Qed.
 
 Definition mon_group_interp :
   Interpretation Monoid.Monoid__repr GroupTest.GroupTest__repr :=
@@ -147,12 +112,21 @@ Definition mon_group_interp :
                                $(prove_sub_spec)$
          )) 0 $(auto)$).
 
+Instance group_mon_ops__instance `{GroupTest.GroupTest} : mon_ops :=
+  map_ops mon_group_interp grp_repr__ops.
+Instance group_mon_model__instance `{GroupTest.GroupTest} : mon_model :=
+  map_model mon_group_interp _ grp_repr__model.
+
+
+
+
 (*
 Definition import_0_0__isoInterp :
   IsoInterpretation Monoid.Monoid__iso GroupTest.GroupTest__iso (proj1_sig mon_group_interp) :=
   toIsoInterp mon_group_interp.
 *)
 
+(*
 Instance import_0_0_instance__T `{GroupTest.GroupTest}
 
 Instance group_mon_T `{T__param:GroupTest.T__class} : Monoid.T__class := T__param.
@@ -178,10 +152,20 @@ Check @test_inst1.
 Set Printing All.
 
 Check @GroupTest.m_zero_right__axiom.
+*)
+
 
 Section GroupTest_Thms.
 Import GroupTest.
 Context `{GroupTest}.
+
+Hint Extern 3 (@Monoid.Monoid _ _ _) =>
+     (unfold mon_T__instance; unfold mon_m_zero__instance; unfold mon_m_plus__instance;
+      unfold group_mon_ops__instance) : typeclass_instances.
+
+Definition blah := left_id_uniq.
+Set Printing All.
+Check blah.
 
 Lemma m_left_id_uniq (x:T) : (forall y, m_plus x y = y) -> x = m_zero.
   apply left_id_uniq.
